Extra/Equiv/Fin.lean
@@ -1,0 +1,62 @@
+/-
+Copyright © 2026 François G. Dorais. All rights reserved.
+Released under Apache 2.0 license as described in the file LICENSE.
+-/
+import Extra.Equiv.Basic
+
+namespace Equiv
+
+def equivEmpty : Equiv (Fin 0) Empty where
+  fwd := Fin.decodeEmpty
+  rev := Fin.encodeEmpty
+  fwd_eq_iff_rev_eq := ⟨by intro | rfl => simp, by intro | rfl => simp⟩
+
+def equivPUnit : Equiv (Fin 1) PUnit where
+  fwd := Fin.decodePUnit
+  rev := Fin.encodePUnit
+  fwd_eq_iff_rev_eq := ⟨by intro h; cases h; simp, by intro | rfl => simp⟩
+
+def equivBool : Equiv (Fin 2) Bool where
+  fwd := Fin.decodeBool
+  rev := Fin.encodeBool
+  fwd_eq_iff_rev_eq := ⟨by intro | rfl => simp, by intro | rfl => simp⟩
+
+def equivOrdering : Equiv (Fin 3) Ordering where
+  fwd := Fin.decodeOrdering
+  rev := Fin.encodeOrdering
+  fwd_eq_iff_rev_eq := ⟨by intro | rfl => simp, by intro | rfl => simp⟩
+
+def equivOption : Equiv (Fin (n+1)) (Option (Fin n)) where
+  fwd x := Fin.decodeOption x
+  rev x := Fin.encodeOption x
+  fwd_eq_iff_rev_eq := ⟨by intro | rfl => simp, by intro | rfl => simp⟩
+
+def equivSum : Equiv (Fin (n+m)) (Sum (Fin n) (Fin m)) where
+  fwd x := Fin.decodeSum x
+  rev x := Fin.encodeSum x
+  fwd_eq_iff_rev_eq := ⟨by intro | rfl => simp, by intro | rfl => simp⟩
+
+def equivProd : Equiv (Fin (n*m)) (Fin n × Fin m) where
+  fwd x := Fin.decodeProd x
+  rev x := Fin.encodeProd x
+  fwd_eq_iff_rev_eq := ⟨by intro | rfl => simp, by intro | rfl => simp⟩
+
+def equivFun : Equiv (Fin (n^m)) (Fin m → Fin n) where
+  fwd x := Fin.decodeFun x
+  rev x := Fin.encodeFun x
+  fwd_eq_iff_rev_eq := ⟨by intro | rfl => simp, by intro | rfl => simp⟩
+
+def equivSigma (f : Fin n → Nat) : Equiv (Fin (Fin.sum f)) ((i : Fin n) × Fin (f i)) where
+  fwd x := Fin.decodeSigma f x
+  rev x := Fin.encodeSigma f x
+  fwd_eq_iff_rev_eq := ⟨by intro | rfl => simp, by intro | rfl => simp⟩
+
+def equivPi (f : Fin n → Nat) : Equiv (Fin (Fin.prod f)) ((i : Fin n) → Fin (f i)) where
+  fwd x := Fin.decodePi f x
+  rev x := Fin.encodePi f x
+  fwd_eq_iff_rev_eq := ⟨by intro | rfl => simp, by intro | rfl => simp⟩
+
+def equivSubtype (P : Fin n → Prop) [DecidablePred P] : Equiv (Fin (Fin.countP (P ·))) { i : Fin n // P i} where
+  fwd x := Fin.decodeSubtype P x
+  rev x := Fin.encodeSubtype P x
+  fwd_eq_iff_rev_eq := ⟨by intro | rfl => simp, by intro | rfl => simp⟩
