Extra/Index/FlatMap.lean
@@ -1,0 +1,67 @@
+import Extra.Index.Basic
+import Extra.Index.Flatten
+import Extra.Index.Map
+
+namespace List.Index
+
+def flatMap (f : α → List β) (k : (i : Index xs) × (Index (f i.val))) :
+    Index (xs.flatMap f) :=
+  flatten ⟨map f k.1, val_map f k.1 ▸ k.2⟩
+
+def unFlatMap (f : α → List β) {xs : List α} (k : Index (xs.flatMap f)) :
+    (i : Index xs) × (Index (f i.val)) :=
+  match unflatten k with
+  | ⟨k₁, k₂⟩ => ⟨unmap f k₁, val_unmap f k₁ ▸ k₂⟩
+
+theorem unFlatMap_flatMap (f : α → List β) {xs : List α} (i : Index xs)
+    (j : Index (f i.val)) : unFlatMap f (flatMap f ⟨i, j⟩) = ⟨i, j⟩ := by
+  simp only [flatMap, unFlatMap]
+  congr
+  · rw [unflatten_flatten, unmap_map]
+  · simp only [eqRec_heq_iff_heq]
+    rw [unflatten_flatten]
+    simp
+
+theorem flatMap_unFlatMap (f : α → List β) {xs : List α} (k : Index (xs.flatMap f)) :
+    flatMap f (unFlatMap f k) = k := by
+  match h : unflatten k with
+  | ⟨i, j⟩ =>
+    rw [unflatten_eq_iff_eq_flatten] at h
+    simp only [flatMap, unFlatMap, h]
+    congr
+    · rw [map_unmap, h, unflatten_flatten]
+    · simp only [eqRec_heq_iff_heq]; rw [h, unflatten_flatten]
+
+theorem flatMap_eq_iff_eq_unFlatMap (f : α → List β) (i : (i : Index xs) × Index (f i.val))
+    (j : Index (xs.flatMap f)) : flatMap f i = j ↔ i = unFlatMap f j := by
+  constructor
+  · intro h; rw [←h, unFlatMap_flatMap]
+  · intro h; rw [h, flatMap_unFlatMap]
+
+theorem unFlatMap_eq_iff_eq_flatMap (f : α → List β) (i : Index (xs.flatMap f))
+    (j : (i : Index xs) × Index (f i.val)) : unFlatMap f i = j ↔ i = flatMap f j := by
+  constructor
+  · intro h; rw [←h, flatMap_unFlatMap]
+  · intro h; rw [h, unFlatMap_flatMap]
+
+def flatMapEquiv (f : α → List β) (xs : List α) :
+    Equiv ((i : Index xs) × Index (f i.val)) (Index (xs.flatMap f)) where
+  fwd := flatMap f
+  rev := unFlatMap f
+  fwd_eq_iff_rev_eq := by
+    intros
+    constructor
+    · intro | rfl => exact unFlatMap_flatMap ..
+    · intro | rfl => exact flatMap_unFlatMap ..
+
+private theorem val_flatMap_eq (f : α → List β) (k : (i : Index xs) × Index (f i.val)) :
+    (flatMap f k).val = (flatten ⟨map f k.1, val_map f k.1 ▸ k.2⟩).val := rfl
+
+theorem val_flatMap (f : α → List β) (k : (i : Index xs) × Index (f i.val)) :
+    (flatMap f k).val = k.snd.val := by
+  simp only [val_flatMap_eq, val_flatten]
+  congr <;> simp [val_map]
+
+theorem val_unFlatMap (f : α → List β)  {xs : List α} (i : Index (xs.flatMap f)) :
+    (unFlatMap f i).snd.val = i.val := by
+  rw [←flatMap_unFlatMap f i, val_flatMap, unFlatMap_flatMap]
